2025/03/05: hoare_while and iter_count

Hoare.v
@@ -74,17 +74,21 @@ Coercion bassn : bexp >-> Assertion.
 Arguments bassn /.
 
 Lemma bexp_eval_true : forall b st,
-  beval st b = true -> (bassn b) st.
+  beval st b = true <-> (bassn b) st.
 Proof.
-  intros b st Hbe.
-  unfold bassn. assumption.  Qed.
+  intros b st. split; intros Hbe; unfold bassn in *; assumption.  
+Qed.
 
 Lemma bexp_eval_false : forall b st,
-  beval st b = false -> ~ ((bassn b) st).
+  beval st b = false <-> ~ ((bassn b) st).
 Proof.
-  intros b st Hbe contra.
+  intros b st. split; intros Hbe. intros contra.
   unfold bassn in contra.
-  rewrite -> contra in Hbe. inversion Hbe.  Qed.
+  rewrite -> contra in Hbe. inversion Hbe.  
+  unfold bassn in Hbe. destruct (beval st b) eqn: Hbeval.
+  - exfalso. apply Hbe. reflexivity.
+  - reflexivity.
+Qed.
 
 Definition assn_sub X a (P:Assertion) : Assertion :=
   fun (st : state) =>
@@ -197,12 +201,293 @@ Proof.
     split; try assumption. intros contra. simpl in contra. rewrite Hb in contra. inversion contra.
 Qed.
 
+Open Scope imp_scope.
+Inductive reduction_in : nat -> (com * state) -> (com * state) -> Prop :=
+  | ri_refl : forall c st, reduction_in 0 (c, st) (c, st)
+  | ri_step : forall c st c' st' c'' st'' n,
+      c / st --c-> c' / st' ->
+      reduction_in n (c', st') (c'', st'') ->
+      reduction_in (S n) (c, st) (c'', st'').
+
+Lemma reduction_in_trans : forall n1 n2 c1 st1 c2 st2 c3 st3,
+  reduction_in n1 (c1, st1) (c2, st2) ->
+  reduction_in n2 (c2, st2) (c3, st3) ->
+  reduction_in (n1 + n2) (c1, st1) (c3, st3).
+Proof.
+  intros. dependent induction H; simpl in *.
+  - assumption.
+  - specialize (IHreduction_in c' st' c2 st2).
+    destruct IHreduction_in; try reflexivity; try assumption.
+    eapply ri_step. apply H. apply ri_refl.
+    eapply ri_step. apply H. eapply ri_step. apply H2. assumption.
+Qed.
+
+Lemma reduction_in_multi_cstep_iff : forall c st c' st',
+  c / st --c->* c' / st' <->
+  exists n, reduction_in n (c, st) (c', st').
+Proof.
+  split; intros.
+  - dependent induction H. exists 0. apply ri_refl.
+    destruct y as [cy sty].
+    specialize (IHmulti cy sty c' st').
+    destruct IHmulti as [n IHmulti]; try reflexivity.
+    exists (S n). eapply ri_step. apply H. assumption.
+  - destruct H as [n H]. dependent induction H.
+    apply multi_refl. eapply multi_step. apply H. apply IHreduction_in.
+    reflexivity. reflexivity.
+Qed.
+
+Lemma com_if_false_rev : forall b c1 c2 st st',
+  TEST b THEN c1 ELSE c2 FI / st --c->* SKIP / st' ->
+  beval st b = false ->
+  c2 / st --c->* SKIP / st'.
+Proof.
+  intros. dependent induction H.
+  inversion H; subst.
+  - specialize (IHmulti b' c1 c2 st st'). destruct IHmulti; try reflexivity.
+    apply bstep_beval_equal in H7. rewrite <- H7. assumption.
+    apply multi_refl. eapply multi_step. apply H2. apply m.
+  - inversion H1.
+  - apply H0.
+Qed.
+
+Lemma com_if_true_rev : forall b c1 c2 st st',
+  TEST b THEN c1 ELSE c2 FI / st --c->* SKIP / st' ->
+  beval st b = true ->
+  c1 / st --c->* SKIP / st'.
+Proof.
+  intros. dependent induction H.
+  inversion H; subst.
+  - specialize (IHmulti b' c1 c2 st st'). destruct IHmulti; try reflexivity.
+    apply bstep_beval_equal in H7. rewrite <- H7. assumption.
+    apply multi_refl. eapply multi_step. apply H2. apply m.
+  - apply H0.
+  - inversion H1.
+Qed.
+
+Lemma com_while_false_eqst : forall b c st st',
+  (WHILE b DO c END) / st --c->* SKIP / st' ->
+  beval st b = false ->
+  st = st'.
+Proof.
+  intros. inversion H; subst. inversion H1; subst.
+  assert (Hfalse := com_if_false _ _ _ _ _ H2 H0).
+  inversion Hfalse; subst; try solve_by_invert. reflexivity.
+Qed.
+
+Inductive iter_count : bexp -> com -> nat -> state -> state -> Prop :=
+  | ic_end : forall b c st, beval st b = false -> iter_count b c 0 st st
+  | ic_step : forall b c st st' st'' n,
+      beval st b = true ->
+      c / st --c->* SKIP / st' ->
+      iter_count b c n st' st'' ->
+      iter_count b c (S n) st st''.
+
+Lemma iter_count_split : forall b c n st st',
+  iter_count b c (S n) st st' ->
+  exists st'', c / st --c->* SKIP / st'' /\ iter_count b c n st'' st'.
+Proof.
+  intros. inversion H. subst. exists st'0. split; assumption.
+Qed.
+
+Definition step_infer {X: Type} (R: relation X) (P: X -> Prop) : Prop :=
+  forall a b, P a -> R a b -> P b.
+
+Lemma multi_infer {X: Type} (R: relation X) (P: X -> Prop) :
+  step_infer R P ->
+  forall a b, P a -> multi R a b -> P b.
+Proof.
+  unfold step_infer. intros Hstep a b HP Hmulti.
+  induction Hmulti; subst; try assumption.
+  assert (Hz := IHHmulti (Hstep x y HP H)). assumption.
+Qed.
+
+Lemma multi_end {X : Type} (R: relation X):
+  forall (x y: X), multi R x y ->
+  x = y \/ (x <> y /\ exists z, multi R x z /\ R z y).
+Proof.
+  intros. dependent induction H.
+  - left. reflexivity.
+  - destruct IHmulti as [IHmulti | [IHmulti_neq [z0 [IHmulti1 IHmulti2]]]];
+    assert (Hexmid := classic (x = z)); destruct Hexmid as [Hexmid | Hexmid];
+    try (left; assumption); right; split; try assumption.
+    subst. exists x. split; try assumption. apply multi_refl.
+    exists z0. split; try assumption. eapply multi_step. apply H. apply IHmulti1. 
+Qed. 
+
+Inductive while_succ : (com * state) -> (com * state) -> Prop :=
+  | ws_self : forall b c st st', while_succ (WHILE b DO c END, st) (WHILE b DO c END, st')
+  | ws_if : forall b b' c st st', 
+    b / st' --b->* b' ->
+    while_succ (WHILE b DO c END, st) (TEST b' THEN c;; WHILE b DO c END ELSE SKIP FI, st')
+  | ws_seq : forall b c c' st st', 
+    while_succ (WHILE b DO c END, st) (c' ;; WHILE b DO c END, st')
+  | ws_skip : forall b c st st',
+    while_succ (WHILE b DO c END, st) (SKIP, st').
+  
+Lemma com_while_succ : forall b c c' st st',
+  (WHILE b DO c END) / st --c->* c' / st' ->
+  while_succ (WHILE b DO c END, st) (c', st').
+Proof.
+  intros. remember (while_succ (WHILE b DO c END, st)) as Hws.
+  assert (Hsi : step_infer cstep Hws). {
+    unfold step_infer. intros. subst. inversion H0; subst; inversion H1; subst.
+    - eapply ws_if. apply multi_refl.
+    - eapply ws_if. eapply multi_trans. apply H6. eapply multi_step. apply H8. apply multi_refl.
+    - eapply ws_seq.
+    - eapply ws_skip.
+    - eapply ws_seq.
+    - eapply ws_self.
+  }
+  assert (Hmi := multi_infer cstep Hws Hsi).
+  assert (Hst : Hws (WHILE b DO c END, st)). { subst. apply ws_self. }
+  eapply Hmi. apply Hst. apply H.
+Qed.
+
+Lemma com_while_false : forall b c st st',
+  (WHILE b DO c END) / st --c->* SKIP / st' ->
+  beval st' b = false.
+Proof.
+  intros. 
+  assert (Hend := multi_end cstep _ _ H).
+  destruct Hend as [Hend_eq | [Hend_neq [z [Hend1 Hend2]]]]; try solve_by_invert.
+  destruct z as [cz stz].
+  assert (Hsucc := com_while_succ _ _ _ _ _ Hend1).
+  inversion Hend2; try (subst; inversion Hsucc); subst.
+  apply bmultistep_beval_equal in H1. simpl in H1. assumption.
+Qed.
+
+Definition is_seq (c : com) : bool :=
+  match c with
+  | CSeq _ _ => true
+  | _ => false
+  end.
+
+Inductive first_iter : (com * state) -> (com * state) -> Prop :=
+  | fi_while : forall b c st, first_iter (WHILE b DO c END, st) (WHILE b DO c END, st)
+  | fi_if : forall b c st b', 
+    b / st --b->* b'
+    -> first_iter (WHILE b DO c END, st) (TEST b' THEN c;; WHILE b DO c END ELSE SKIP FI, st)
+  | fi_seq : forall b c st c' st',
+    beval st b = true
+    -> c / st --c->* c' / st'
+    -> first_iter (WHILE b DO c END, st) ((c' ;; WHILE b DO c END), st').
+
+Definition seq_left (c : com) : com :=
+  match c with
+  | CSeq c1 _ => c1
+  | _ => SKIP
+  end.
+
+Inductive pwhile : (com * state) -> (com * state) -> Prop :=
+  | pw_firstiter : forall b c st c' st',
+    ((WHILE b DO c END) / st --c->* c' / st')
+    /\ first_iter (WHILE b DO c END, st) (c', st')
+    -> pwhile (WHILE b DO c END, st) (c', st')
+  | pw_nseq : forall b c st c' st',
+    ((WHILE b DO c END) / st --c->* c' / st')
+    /\ is_seq c' = false
+    /\ (exists n, iter_count b c n st st')
+    -> pwhile (WHILE b DO c END, st) (c', st')
+  | pw_seq : forall b c st c' st', 
+    ((WHILE b DO c END) / st --c->* c' / st')
+    /\ is_seq c' = true
+    /\ (exists st'', ( c / st'' --c->* (seq_left c') / st' /\ exists n, iter_count b c n st st'' /\ beval st'' b = true ))
+    -> pwhile (WHILE b DO c END, st) (c', st').
+
+Fixpoint com_size (c : com) : nat :=
+  match c with
+  | SKIP => 1
+  | CAss _ _ => 1
+  | CSeq c1 c2 => (com_size c1) + (com_size c2)
+  | CIf _ c1 c2 => (com_size c1) + (com_size c2)
+  | CWhile _ c => (com_size c)
+  | CAwait _ c => (com_size c)
+  | CCoroutine c1 c2 => (com_size c1) + (com_size c2)
+  end.
+
+Lemma com_size_gt_0 : forall c,
+  com_size c > 0.
+Proof.
+  intros. induction c; simpl; lia.
+Qed.
+
+Lemma com_seq_not_nested : forall c1 c2,
+  ~ (c2 = (c1 ;; c2)).
+Proof.
+  intros. intros contra.
+  assert (Heqsize : com_size c2 = com_size (c1 ;; c2)). {
+    rewrite <- contra. reflexivity.
+  }
+  simpl in Heqsize.
+  assert (Hgt := com_size_gt_0 c2).
+  assert (Hgt' := com_size_gt_0 c1).
+  destruct (com_size c2) eqn: Hsize; simpl in *.
+  - inversion Hgt.
+  - destruct (com_size c1) eqn: Hsize'; simpl in *.
+    + inversion Hgt'.
+    + lia.
+Qed.
+
+Lemma com_seq_left : forall c1 c1' c2 st st',
+  c1 / st --c->* c1' / st' ->
+  (c1 ;; c2) / st --c->* (c1' ;; c2) / st'.
+Proof.
+  intros. dependent induction H. apply multi_refl.
+    destruct y as [cy sty]. specialize (IHmulti cy c1' sty st').
+    eapply multi_step. apply CS_SeqStep. apply H. apply IHmulti; reflexivity.
+Qed.
+
+Lemma com_while_count_rev : forall b c n st st',
+  iter_count b c n st st' ->
+  WHILE b DO c END / st --c->* SKIP / st'.
+Proof.
+  intros. dependent induction H.
+  - eapply multi_step. ector.
+    apply bmultistep_beval_iff in H.
+    assert (Hfwd := com_if_fwd _ _ (c;; WHILE b DO c END) SKIP _ H).
+    eapply multi_trans. apply Hfwd. eapply multi_step. apply CS_IfFalse.
+    apply multi_refl.
+  - eapply multi_step. ector.
+    apply bmultistep_beval_iff in H.
+    assert (Hfwd := com_if_fwd _ _ (c;; WHILE b DO c END) SKIP _ H).
+    eapply multi_trans. apply Hfwd. eapply multi_step. apply CS_IfTrue.
+    eapply com_seq_compose. apply H0. apply IHiter_count.
+Qed.
+
+Lemma com_while_count : forall b c st st',
+  WHILE b DO c END / st --c->* SKIP / st'
+  -> exists n,  iter_count b c n st st'.
+Proof.
+  intros. 
+Admitted.
+
+
 (* 2.4 iteration *)
 Theorem hoare_while : forall P (b:bexp) c,
   {{P /\ b}} c {{P}} ->
   {{P}} WHILE b DO c END {{P /\ ~ b}}.
 Proof.
-  Admitted.
+  unfold hoare_triple. intros P b c Hhoare st st' Heval HP.
+  assert (Hcount := com_while_count b c st st' Heval). 
+  destruct Hcount as [n Hcount].
+  generalize dependent st. generalize dependent st'.
+  induction n; intros.
+  - inversion Hcount. subst. split; try apply bexp_eval_false; try assumption.
+  - destruct (beval st b) eqn: Hb.
+    + assert (Hc := iter_count_split _ _ _ _ _ Hcount).
+      destruct Hc as [st'' [Hc Hcount']].
+      assert (Hwhile := com_while_count_rev b c n st'' st' Hcount').
+      simpl in Hhoare.
+      assert (Hconj : P st /\ beval st b = true). { split; assumption. }
+      assert (HPst'' := Hhoare _ _ Hc  Hconj).
+      assert (IHn' := IHn _ _ Hwhile HPst'' Hcount').
+      assumption.
+    + inversion Heval. subst. inversion H. subst.
+      assert (Hfalse := com_if_false_rev _ _ _ _ _ H0 Hb).
+      inversion Hfalse; subst; try solve_by_invert.
+      apply bexp_eval_false in Hb. split; assumption.
+Qed.
 
 (* 3.2 await *)
 Theorem hoare_await : forall P Q (b:bexp) c,
